reorganize files and namespaces

RowPredicates/Label.lean
@@ -1,17 +1,15 @@
 module
 
-
 @[expose] public section
 
 namespace Label
 
 inductive Label : Type where
-  | label (s : String)  : Label
-  | LVar (name: String) : Label
+  | explicit (s : String)  : Label
+  | lVar (name: String) : Label
 
 inductive Label.concrete : Label -> Prop where
- | literal : Label.concrete (.label s)
+ | literal : Label.concrete (.explicit s)
 
+-- Equality of labels is purely syntactic
 deriving instance BEq, DecidableEq, Ord, ReflBEq, LawfulBEq for Label
-
--- Boolean equality of labels is purely syntactic
