RowPredicates/Context.lean
@@ -1,0 +1,46 @@
+module
+
+public import RowPredicates.Kind
+public import RowPredicates.Label
+public import RowPredicates.WF
+public import Std.Data.HashMap
+
+
+namespace Context
+
+open Kind Label
+
+
+def KindType (k : Kind) : Type :=
+  match k with
+  | .KRow => WF.Row
+  | .KTy => WF.Ty
+  | .KLabel => Label
+
+def KindContext : Kind -> Type := λ k => Std.HashMap String (KindType k)
+
+def KindContext.empty {k : Kind} : KindContext k := .emptyWithCapacity
+
+structure Context where
+  rowContext : KindContext .KRow := .empty
+  typeContext : KindContext .KTy := .empty
+  labelContext : KindContext .KLabel := .empty
+  getContext (k: Kind) : KindContext k :=
+      match k with
+      | .KRow => rowContext
+      | .KTy => typeContext
+      | .KLabel => labelContext
+  get {k : Kind} (s: String) : Option (KindType k) := (getContext k).get? s
+  insert {k : Kind} (s: String) : Option (KindType k) := (getContext k).get? s
+
+def Context.empty : Context := {}
+
+inductive WithContext {c : Context} (T : Type): Type where
+| wrap : T -> WithContext T
+
+def unwrap : WithContext (c := c) T -> T
+| .wrap x => x
+
+def RowWithContext {c : Context} := WithContext (c := c) WF.Row
+def TyWithContext {c : Context} := WithContext (c := c) WF.Ty
+def LabelWithContext {c : Context} := WithContext (c := c) Label
