RowPredicates/Pre.lean
@@ -1,0 +1,96 @@
+module
+
+public import RowPredicates.Label
+
+@[expose] public section
+
+namespace Pre
+
+open Label
+
+mutual
+inductive Row : Type where
+  | empty : Row -- (Identity for Concat)
+  | rVar : String -> Row
+  | extend : Row -> Label -> Ty -> Row
+
+inductive Ty : Type where
+  | TVar (name : String) : Ty
+  | TFun (arg: Ty) (ret: Ty) : Ty
+  | Singleton : Label -> Ty
+  | Pi : Row -> Ty
+  | Sigma : Row -> Ty
+end
+
+def Row.type_at (r: Row) (l: Label) : Option Ty :=
+  match r with
+    | .empty => .none
+    | .rVar _ => .none
+    | .extend r' l' t =>
+        if l = l'
+        then .some t
+        else type_at r' l
+
+inductive Row.lack : Row -> (Label) -> Prop where
+  | empty : Row.lack .empty l
+  | rVar : l ≠ l -> Row.lack (Row.rVar s) l
+  | extend : Row.lack r l -> l ≠ l' -> Row.lack (extend r l' t) l
+
+theorem Row.lack_extend_lack : lack (.extend r l' t) l -> lack r l
+| .extend h _ => h
+
+inductive Row.has_label : Row -> Label -> Prop where
+  | first : has_label (.extend r l _) l
+  | extend : (has_label r l) -> has_label (.extend r _ _) l
+
+theorem Row.has_label_neg_lack (h: has_label r l): ¬lack r l :=
+  λ hn =>
+    match h with
+    | .first => match hn with
+      | .extend _ _ => by contradiction
+    | .extend h' =>  (has_label_neg_lack h' (lack_extend_lack hn))
+
+inductive Row.disjoint : Row -> Row -> Prop where
+  | refl : disjoint .empty .empty
+  | extend : disjoint r1 r2 -> l1 ≠ l2 -> r1.lack l2 -> r2.lack l1 -> disjoint (.extend r1' l1 t1) (.extend r2' l2 t2)
+
+
+def Row.le (r1 r2: Row) : Prop :=
+  forall (l : Label), r2.has_label l -> r1.has_label l ∧ (type_at r1 l) = (type_at r2 l)
+
+
+
+theorem Row.disjoint_symm {r1 r2 : Row} (h: Row.disjoint r1 r2) : Row.disjoint r2 r1 :=
+  match h with
+  | .refl => .refl
+  | .extend a b c d => by
+    apply Row.disjoint.extend
+    constructor
+    symm
+    exact b
+    exact .empty
+    exact .empty
+
+inductive Row.unique_labels : Row -> Prop where
+  | empty : unique_labels .empty
+  | rVar : unique_labels (.rVar s)
+  | extend : unique_labels r -> lack r l -> unique_labels (extend r l t)
+
+theorem Row.unique_labels_lack_extend : Row.unique_labels (.extend r l t) -> Row.lack r l := by
+  intro h
+  cases h
+  assumption
+
+theorem Row.unique_labels_extend {pr : Row} {l t} : Row.unique_labels (.extend pr l t) -> Row.unique_labels pr := by
+  cases pr <;> intro h
+  apply unique_labels.empty
+  apply unique_labels.rVar
+  cases h ;
+  assumption
+
+-- Row is concrete (Has explicit labels and is not a variable)
+-- `concrete` is shallow, so it imposes no constraints on structures nested inside the row
+inductive Row.concrete : Row -> Prop where
+  | empty : concrete .empty
+  | extend : concrete r -> Label.concrete l -> lack r l -> concrete (extend r l t)
+
