RowPredicates/Pred.lean
@@ -1,0 +1,32 @@
+module
+
+public import RowPredicates.Kind
+public import RowPredicates.Label
+public import RowPredicates.Term
+public import RowPredicates.WF
+
+@[expose] public section
+
+namespace Pred
+
+open Label Kind Term WF Pred
+
+-- This should (maybe?) bundle evidence eventually
+inductive Pred : Type where
+  | Leq (x: WF.Row) (y: WF.Row) : Pred
+    -- Garrett-style 3-place concatenation predicate
+    -- x + y ~ z
+  | Concat (x: WF.Row) (y: WF.Row) (z: WF.Row) :Pred
+  | Eq (x: WF.Row) (y: WF.Row) : Pred
+
+inductive PredTerm : Type where
+  | Leq : Term -> Term -> PredTerm
+  | Eq : Term -> Term -> PredTerm
+    -- Garrett-style 3-place concatenation predicate
+    -- x + y ~ z
+  | Concat : Term -> Term -> Term -> PredTerm
+
+-- inductive PredTerm.WK : PredTerm -> Prop where
+--   | Leq : Term.WK x KRow -> Term.WK y KRow -> PredTerm.WK (PredTerm.Leq x y)
+--   | Eq : Term.WK x KRow -> Term.WK y KRow -> Term.WK y KRow -> PredTerm.WK (PredTerm.Concat x y z)
+--   | Concat : Term.WK x KRow -> Term.WK y KRow -> Term.WK y KRow -> PredTerm.WK (PredTerm.Concat x y z)
