RowPredicates/Term.lean
@@ -1,0 +1,35 @@
+module
+
+public import RowPredicates.Kind
+public import RowPredicates.Label
+
+namespace Term
+
+@[expose] public section
+
+open Label Kind
+
+inductive Term : Type where
+  | RVar : (name : String) -> Term
+  | TVar : (name : String) -> Term
+  | TFun : Term -> Term -> Term
+  | Field : Label -> Term -> Term
+  | Row : List Term -> Term
+  | Singleton : Label -> Term
+  | Pi : Term -> Term
+  | Sigma : Term -> Term
+  -- leaving off type-level functions now to keep it simple
+  -- | TApp
+  -- | TLam
+
+-- Assert that all fields in the field list have a term which satisfies the given propositional predicate
+inductive AllFields : (Pred: Term -> Prop) -> List Term -> Prop where
+  | Nil : (AllFields Pred [])
+  | Cons : Pred t -> AllFields Pred fields -> (AllFields Pred ((Term.Field l t)::fields))
+
+-- Well-Kindedness Judgement
+inductive Term.WK : Term -> Kind -> Prop where
+  | RVar : (name : String) -> WK (.RVar name) KRow
+  | TVar : (name : String) -> WK (.TVar name) KTy
+  | TFun : (Term.WK arg Ty) -> (Term.WK ret Ty) -> (Term.WK (TFun arg ret) Ty)
+  | Row : (fields: List Term) -> (AllFields (λ t => Term.WK t .KTy) fields) -> (Term.WK (Row fields) KRow)
