RowPredicates/WF.lean
@@ -1,0 +1,200 @@
+module
+public import RowPredicates.Pre
+public import RowPredicates.Label
+
+@[expose] public section
+
+namespace WF
+
+open Pre Label WF
+
+
+-- Interdefined Well-formedness rules for Pre.Row and Pre.Ty
+mutual
+inductive WF_Ty : (inner: Pre.Row) -> Prop where
+  | empty : WF_Ty .empty
+  | rVar : WF_Ty (.rVar s)
+  | extend : WF_Ty r -> Pre.Row.unique_labels r -> r.lack l -> (WF_Row t) -> WF_Ty (.extend r l t)
+
+inductive WF_Row : (inner: Pre.Ty) -> Prop where
+  | TVar : WF_Row (.TVar s)
+  | TFun : WF_Row arg -> WF_Row ret -> WF_Row (.TFun (arg: Pre.Ty) (ret: Pre.Ty))
+  | Singleton : WF_Row (.Singleton l)
+  | Pi : WF_Ty r -> WF_Row (.Pi r)
+  | Sigma : WF_Ty r -> WF_Row (.Sigma r)
+end
+
+-- TODO set up wellfounded induction over Rows and Tys
+structure Row : Type where
+  inner : Pre.Row
+  wf : WF_Ty inner
+-- Row must be implemented on top of Pre.Row and bundle well-formedness invariant
+
+structure Ty : Type where
+  inner : Pre.Ty
+  wf : WF_Row inner
+
+def Row.unique_labels : Row -> Prop
+  | .mk inner _ => inner.unique_labels
+
+-- A row lacks a label iff the inner (well-formed) pre-row lacks that label
+def Row.lack : Row -> Label -> Prop
+  | ⟨inner, _⟩, l => inner.lack l
+
+def Row.has_label : Row -> Label -> Prop
+  | ⟨inner, _⟩, l => inner.has_label l
+
+def Row.disjoint : Row -> Row -> Prop
+  | ⟨innerL, _⟩, ⟨innerR, _⟩ => innerL.disjoint innerR
+
+def Row.concrete : Row -> Prop
+  | ⟨inner, _⟩ => inner.concrete
+
+
+def Row.type_at_helper (r : Pre.Row) (l : Label) (h : WF_Ty r): Option Ty :=
+  match r with
+  | .empty => .none
+  | .rVar _ => .none
+  | .extend r' l' t =>
+     if l = l'
+      then .some {inner := t, wf := (by cases h ; assumption)}
+      else type_at_helper r' l (by cases h ; assumption)
+
+def Row.type_at : Row -> Label -> Option Ty
+  | ⟨inner, wf⟩, l => type_at_helper inner l wf
+
+
+def Row.le (a b : Row) : Prop :=
+  a.inner.le b.inner
+
+theorem lacks_extend_lacks {r: Pre.Row} {l1 l2: Label} {t: Pre.Ty} (h_lack: Pre.Row.lack (r.extend l2 t) l1) : Pre.Row.lack r l1 :=
+  match h_lack with
+  | .extend h' _ => h'
+
+instance : LE Row where
+  le := Row.le
+
+theorem Row.le_inner_has_label {r1 r2 : Row} {l : Label } (h_le : r1 ≤ r2) (h_has : r2.inner.has_label l) : r1.inner.has_label l := by
+  simp [(.≤.), Row.le, Pre.Row.le] at h_le
+  apply (h_le _ h_has).left
+
+theorem Row.le_trans (r1 r2 r3 : Row) (h_1_2 : r1 ≤ r2) (h_2_3 : r2 ≤ r3) : r1 ≤ r3 :=
+  λ l h => by
+    apply And.intro
+    case left =>
+      apply le_inner_has_label h_1_2 (le_inner_has_label h_2_3 h)
+    case right =>
+      simp [(.≤.),Row.le,Pre.Row.le] at *
+      grind
+
+theorem Row.le_refl : ∀ (x : Row), x ≤ x :=
+  λ _ _ h => And.intro h rfl
+
+instance : Std.IsPreorder Row where
+  le_refl := Row.le_refl
+  le_trans := Row.le_trans
+
+def Ty.TVar (s : String) : Ty :=
+  ⟨Pre.Ty.TVar s, WF_Row.TVar⟩
+
+def Ty.TFun (t1 t2 : Ty) : Ty :=
+  ⟨Pre.Ty.TFun t1.inner t2.inner, WF_Row.TFun t1.wf t2.wf⟩
+
+def Ty.Singleton (l : Label) : Ty :=
+  {
+    inner := Pre.Ty.Singleton l,
+    wf := WF_Row.Singleton
+  }
+
+def Ty.Pi (r : Row) : Ty :=
+  {
+    inner := Pre.Ty.Pi r.inner,
+    wf := WF_Row.Pi r.wf
+  }
+
+def Ty.Sigma (r : Row) : Ty :=
+  {
+    inner := Pre.Ty.Sigma r.inner,
+    wf := WF_Row.Sigma r.wf
+  }
+
+
+mutual
+
+inductive Ty.Equiv : Ty  -> Ty  -> Prop where
+  | TVar : Ty.Equiv (Ty.TVar s) (Ty.TVar s)
+  | Singleton : Ty.Equiv (Ty.Singleton l) (Ty.Singleton l)
+  | Pi : Row.Equiv r1 r2 -> Ty.Equiv (Ty.Pi r1) (Ty.Pi r2)
+  | Sigma : Row.Equiv r1 r2 -> Ty.Equiv (Ty.Sigma r1) (Ty.Sigma r2)
+  | TFun : Ty.Equiv a1 a2 -> Ty.Equiv r1 r2 -> Ty.Equiv (Ty.TFun a1 r1) (Ty.TFun a2 r2)
+
+inductive Row.Equiv : Row  -> Row  -> Prop where
+  | mk {a b : Row} : a ≤ b ∧ b ≤ a -> Row.Equiv a b
+end
+
+theorem Row.Equiv.refl : ∀ r: Row, r.Equiv r :=
+  λ _ => .mk (And.intro
+          (instIsPreorderRow.le_refl _)
+          (instIsPreorderRow.le_refl _))
+
+theorem Row.Equiv.symm : ∀ {x y : Row}, x.Equiv y → y.Equiv x :=
+  λ h =>
+    match h with
+    | .mk (And.intro l r) => .mk (And.intro r l)
+
+theorem Row.Equiv.trans : ∀ {x y z: Row}, x.Equiv y → y.Equiv z → x.Equiv z := by
+  intro x y z h_x_y h_y_z
+  apply Equiv.mk
+  apply And.intro <;>
+    cases h_x_y <;> cases h_y_z <;>
+    simp [.≤.,Row.le,Pre.Row.le] at * <;>
+    grind
+
+theorem Ty.Equiv.refl : ∀ x, Ty.Equiv x x :=
+  λ x =>
+      match x with
+      | .TVar _ => .TVar
+      | .Singleton _ => .Singleton
+      | ⟨.TFun arg ret, WF_Row.TFun wf_a wf_r⟩ =>
+        @Equiv.TFun ⟨arg,wf_a⟩ ⟨arg,wf_a⟩ ⟨ret, wf_r⟩ ⟨ret, wf_r⟩ (.refl _) (.refl _)
+      | ⟨.Pi r, WF_Row.Pi wf_r⟩ =>
+        @Equiv.Pi ⟨r, wf_r⟩ ⟨r, wf_r⟩ (Row.Equiv.refl _)
+      | ⟨.Sigma r, WF_Row.Sigma wf_r⟩ =>
+        @Equiv.Sigma ⟨r, wf_r⟩ ⟨r, wf_r⟩ (Row.Equiv.refl _)
+
+theorem Ty.Equiv.symm : ∀ {x y : Ty}, x.Equiv y → y.Equiv x :=
+  λ h =>
+    match h with
+    | .TVar => Ty.Equiv.TVar
+    | .Singleton => .Singleton
+    | .TFun h1 h2 => .TFun (Ty.Equiv.symm h1) (Ty.Equiv.symm h2)
+    | .Pi h => .Pi (Row.Equiv.symm h)
+    | .Sigma h => .Sigma (Row.Equiv.symm h)
+
+theorem Ty.Equiv.trans : ∀ {x y z : Ty}, x.Equiv y → y.Equiv z → x.Equiv z :=
+  @λ x y z h1 h2 =>
+    match x, y, z with
+    | .TVar x', .TVar y', .TVar z' =>
+      by cases h1 ; cases h2; apply Equiv.refl
+    | .Singleton x', .Singleton y', .Singleton z' =>
+      by cases h1 ; cases h2; apply Equiv.refl
+    | ⟨.TFun _ _, _⟩, _, _ =>
+        match h1, h2 with
+        | @Equiv.TFun ⟨_,_⟩ ⟨_,_⟩ ⟨_,_⟩ ⟨_,_⟩ h1a h1r, Equiv.TFun h2a h2r =>
+          Equiv.TFun (Ty.Equiv.trans h1a h2a) (Ty.Equiv.trans h1r h2r)
+    | ⟨.Pi _, _⟩, _, _ =>
+      match h1, h2 with
+      | @Equiv.Pi _ ⟨_, _⟩ h_xy, Equiv.Pi h_yz => Ty.Equiv.Pi (Row.Equiv.trans h_xy h_yz)
+    | ⟨.Sigma _, _⟩, _, _ =>
+      match h1, h2 with
+      | @Equiv.Sigma _ ⟨_, _⟩ h_xy, Equiv.Sigma h_yz => Ty.Equiv.Sigma (Row.Equiv.trans h_xy h_yz)
+
+-- This definition of equivalence is syntactic, up to reordering of fields
+-- Equivalence of rows with respect to a context or substitution will be defined over quotients of well-formed rows and types
+instance : Setoid Ty where
+  r := Ty.Equiv
+  iseqv := ⟨.refl, .symm, .trans⟩
+
+instance : Setoid Row where
+  r := Row.Equiv
+  iseqv := ⟨.refl, .symm, .trans⟩
